Using Finset instead of FinEum
- Rewrote every definition to use a finset instead of FinEnum

lean4/Automaton/DFA/Basic.lean
@@ -6,6 +6,7 @@ import Mathlib.Data.Fintype.Basic
 import Mathlib.Data.Fintype.List
 import Mathlib.Data.Vector.Basic
 import Mathlib.Data.List.Card
+import Automaton.Finset.Basic
 
 /-!
   This file contains the definition of a DFA as well as a few fundamental operations it can do
@@ -24,69 +25,62 @@ import Mathlib.Data.List.Card
 namespace DFA
 
 
-structure DFA (σ : Type _) where
-  q : Type _             -- states
-  init : q               -- initial state
-  fs : Finset q          -- accepting states
-  δ : q → σ → q          -- transition function
-  [fq : FinEnum q]
-  [fσ : FinEnum σ]
+structure DFA (σ : Type _) (q : Type _) where
+  σs : Finset σ    -- alphabet
+  qs : Finset q    -- states
+  init : qs        -- initial state
+  fs : Finset qs   -- accepting states
+  δ : qs → σs → qs -- transition function
+  [dq : DecidableEq q]
+  [dσ : DecidableEq σ]
 
-variable {σ : Type _} [fσ : FinEnum σ] (r s t : DFA σ)
+variable {σ : Type _} {q : Type _} (r s t : DFA σ q) [DecidableEq σ] [DecidableEq q]
 
-instance : FinEnum t.q := t.fq
+instance : DecidableEq t.σs := by infer_instance
+instance : DecidableEq t.qs := by infer_instance
 
 -- ToString
-
--- if there's enough elements to map them to a-z, do it
--- otherwise map to numbers (26 - size of alphabet, + 97 to get ascii value)
-def symbolFormat : σ → String :=
-  if fσ.card ≤ 26 then  (fun e => String.singleton (Char.ofNat (fσ.equiv.toFun e + 97)))
-  else (fun e => toString (fσ.equiv.toFun e))
-
-def stateFormat {t : DFA σ} : t.q → String := (fun e => toString (t.fq.equiv.toFun e))
-
-instance : ToString (DFA σ) where
+instance [ToString σ] [ToString q] [fσ : FinEnum σ] [fq : FinEnum q] : ToString (DFA σ q) where
   toString t := by
-   have s : List String := (t.fσ.toList).map symbolFormat
-   have q : String := stateFormat t.init
-   have qs : List String :=  (t.fq.toList).map stateFormat
-   have fs : List String := ((t.fq.toList).filter (fun e => e ∈ t.fs)).map stateFormat
-   have δ : List String := (t.fq.toList).map (fun x => String.join ((t.fσ.toList).map (fun y => "("++stateFormat x ++ "×" ++ symbolFormat y ++ ")→"++ stateFormat (t.δ x y) ++ " ")))
-   exact "Σ: " ++ String.join (s.map (fun e => e++" ")) ++ "\n" ++
-         "Q: " ++ String.join (qs.map (fun e => e++" ")) ++ "\n" ++
-         "δ: " ++ String.join (δ.map (fun e => "\n"++e)) ++ "\n" ++
-         "q₀: " ++ q ++ "\n" ++
-         "F: " ++ String.join (fs.map (fun e => e++" ")) ++ "\n"
-         
+    have s : List String := (fσ.toList).map toString
+    have q : String := toString t.init
+    have qs : List String :=  (fq.toList).map toString
+    have fs : List String := ((fq.toList).filter (fun e => e ∈ t.fs.map ⟨ fun a => a.1 , by simp [Function.Injective]⟩)).map toString
+    have δ : List String := (fq.toList).map (fun a => String.join ((fσ.toList).map (fun b => if h : a ∈ t.qs ∧ b ∈ t.σs then "("++ toString a ++ "×" ++ toString b ++ ")→" ++ toString (t.δ ⟨a , h.1⟩ ⟨b , h.2⟩) ++ " " else "")))
+    exact "Σ: { " ++ String.join (s.map (fun e => e++" ")) ++ "}\n" ++
+          "Q: { " ++ String.join (qs.map (fun e => e++" ")) ++ "}\n" ++
+          "δ: " ++ String.join (δ.map (fun e => "\n   "++e)) ++ "\n" ++
+          "q₀: " ++ q ++ "\n" ++
+          "F: { " ++ String.join (fs.map (fun e => e++" ")) ++ "}\n"
+
 
 -- δ* function
 -- the state reached after following all transitions given a word
 -- the first letter in list is the last character consumed
 @[simp]
-def δ_star' (q : t.q) : (w : word σ) → t.q
+def δ_star' (q : t.qs) : (w : word t.σs) → t.qs
   | [] => q
-  | e :: es => δ_star' (t.δ q e) es 
+  | e :: es => δ_star' (t.δ q e) es
 
 
-def δ_star : (w : word σ) → t.q := δ_star' t t.init
+def δ_star : (w : word t.σs) → t.qs := δ_star' t t.init
 
 -- whether a DFA accepts a word
 @[simp]
-def dfa_accepts : (w : word σ) → Prop := by
+def dfa_accepts : (w : word t.σs) → Prop := by
   intro w
   exact δ_star t w ∈ t.fs
 
-def dfaLang : Lang σ := fun w => dfa_accepts t w
+def dfaLang : Lang t.σs := fun w => dfa_accepts t w
 
 
 -- all states reachable from current state
-inductive reachable (q : t.q) : t.q → Prop where
+inductive reachable (q : t.qs) : t.qs → Prop where
   | base : reachable q q
-  | step (q' : t.q) : reachable q q' → ∀ e : σ , reachable q (t.δ q' e)
+  | step (q' : t.qs) : reachable q q' → ∀ e : t.σs , reachable q (t.δ q' e)
 
 
-theorem reachable_trans' (a b : t.q) : reachable t a b → (c : t.q) → reachable t b c → reachable t a c := by
+theorem reachable_trans' (a b : t.qs) : reachable t a b → (c : t.qs) → reachable t b c → reachable t a c := by
   intro h
   induction h with
   | base => intro c ac; exact ac
@@ -94,63 +88,34 @@ theorem reachable_trans' (a b : t.q) : reachable t a b → (c : t.q) → reachab
                      apply s
                      induction qec with
                      | base => apply reachable.step; exact reachable.base
-                     | step q' _ e' s' => apply reachable.step; exact s' 
+                     | step q' _ e' s' => apply reachable.step; exact s'
 
-theorem reachable.trans (a b c : t.q) : reachable t a b → reachable t b c → reachable t a c := by
+theorem reachable.trans (a b c : t.qs) : reachable t a b → reachable t b c → reachable t a c := by
   intro a
   apply reachable_trans'
   exact a
 
 -- DFA language is decidable
-instance decidableLang (w : word σ) : Decidable (dfa_accepts t w) := by
+instance decidableLang (w : word t.σs) : Decidable (dfa_accepts t w) := by
   simp only [dfa_accepts]
-  have : DecidableEq t.q := by exact t.fq.decEq  
   apply Finset.decidableMem
-  
--- equality of DFAs
-def eq : Prop := ∀ w : word σ , dfa_accepts t w ↔ dfa_accepts s w
-
-private theorem eq.refl : eq t t := by
-  intro w
-  apply Iff.intro <;> (intro ; assumption) 
-
-private theorem eq.trans : eq t s → eq s r → eq t r := by
-  intro eq₁ eq₂
-  intro w
-  apply Iff.intro
-  · intro r
-    apply (Iff.mp (eq₁ w))
-    apply (Iff.mp (eq₂ w))
-    exact r
-  · intro t
-    apply (Iff.mpr (eq₂ w))
-    apply (Iff.mpr (eq₁ w))
-    exact t
-
-private theorem eq.sym : eq t s → eq s t := by
-  intro h
-  intro w
-  apply Iff.intro 
-  <;> intro 
-  <;> (first | apply (Iff.mp (h w)) | apply (Iff.mpr (h w))) 
-  <;> assumption
 
 
 -- dfa accepts nil iff init is final
 theorem dfa_accepts_nil_iff_final : dfa_accepts t [] ↔ t.init ∈ t.fs := by
-  apply Iff.intro 
-  <;> intro h 
+  apply Iff.intro
+  <;> intro h
   <;> (first | simp [dfa_accepts])
   <;> exact h
 
-lemma δ_δ_star'_concat_eq_δ_star' : (q : t.q) → DFA.δ t (δ_star' t q l) a = δ_star' t q (l ++ [a]) := by
+lemma δ_δ_star'_concat_eq_δ_star' : (q : t.qs) → DFA.δ t (δ_star' t q l) a = δ_star' t q (l ++ [a]) := by
   induction l with
   | nil => simp
   | cons e es s => intro q
                    simp only [δ_star',List.append_eq]
                    apply s (DFA.δ t q e)
 
-theorem δ_star_append_eq (r : word σ) : (l : word σ) → δ_star t (l++r) = δ_star' t (δ_star t l) r := by
+theorem δ_star_append_eq (r : word t.σs) : (l : word t.σs) → δ_star t (l++r) = δ_star' t (δ_star t l) r := by
   induction r with
   | nil => simp
   | cons a as s => intro l
@@ -160,23 +125,23 @@ theorem δ_star_append_eq (r : word σ) : (l : word σ) → δ_star t (l++r) = �
 
 
 
-lemma δ_star'_reachable (w : word σ) (q : t.q) : (q' : t.q) → reachable t q q' → reachable t q (δ_star' t q' w) := by
+lemma δ_star'_reachable (w : word t.σs) (q : t.qs) : (q' : t.qs) → reachable t q q' → reachable t q (δ_star' t q' w) := by
   induction w with
   | nil => simp [δ_star]
-  | cons e es s => intro q' rq' 
+  | cons e es s => intro q' rq'
                    rw [δ_star']
                    apply s
                    apply reachable.step
                    exact rq'
-  
 
-theorem accepts_from_state_if (w : word σ) (q : t.q) : (∀ q' : t.q , (reachable t q q' → q' ∈ t.fs)) → δ_star' t q w ∈ t.fs := by
+
+theorem accepts_from_state_if (w : word t.σs) (q : t.qs) : (∀ q' : t.qs , (reachable t q q' → q' ∈ t.fs)) → δ_star' t q w ∈ t.fs := by
   intro q'
   apply q'
   apply δ_star'_reachable
-  exact reachable.base 
+  exact reachable.base
 
-theorem state_reachable_iff (q q' : t.q) : reachable t q q' ↔ ∃ w : word σ , δ_star' t q w = q' := by
+theorem state_reachable_iff (q q' : t.qs) : reachable t q q' ↔ ∃ w : word t.σs , δ_star' t q w = q' := by
   apply Iff.intro
   · intro rq'
     induction rq' with
@@ -188,12 +153,12 @@ theorem state_reachable_iff (q q' : t.q) : reachable t q q' ↔ ∃ w : word σ 
   · intro ex
     apply Exists.elim ex
     intro w δ'
-    simp only [δ_star'] at δ' 
+    simp only [δ_star'] at δ'
     rw [←δ']
     apply δ_star'_reachable
-    exact reachable.base 
+    exact reachable.base
 
-theorem accepts_prefix_if (l r : word σ) : (∀ q' : t.q , (reachable t (δ_star t l) q' → q' ∈ t.fs)) → dfa_accepts t (l ++ r) := by
+theorem accepts_prefix_if (l r : word t.σs) : (∀ q' : t.qs , (reachable t (δ_star t l) q' → q' ∈ t.fs)) → dfa_accepts t (l ++ r) := by
   intro fa
   rw [dfa_accepts,δ_star_append_eq]
   apply accepts_from_state_if
@@ -204,7 +169,7 @@ theorem accepts_prefix_if (l r : word σ) : (∀ q' : t.q , (reachable t (δ_sta
 -- To prove that DFA accepts any word starting with a prefix
 -- If after l, a state is reached from which all combinations of transitions lead
 -- to a final state, it always
-theorem accepts_prefix_iff (p : word σ) : dfa_accepts t p ∧ (∀ q' : t.q , (reachable t (δ_star t p) q' → q' ∈ t.fs)) ↔ ∀ s : word σ , dfa_accepts t (p ++ s) := by
+theorem accepts_prefix_iff (p : word t.σs) : dfa_accepts t p ∧ (∀ q' : t.qs , (reachable t (δ_star t p) q' → q' ∈ t.fs)) ↔ ∀ s : word t.σs , dfa_accepts t (p ++ s) := by
   apply Iff.intro
   · intro h s
     apply accepts_prefix_if
@@ -223,17 +188,17 @@ theorem accepts_prefix_iff (p : word σ) : dfa_accepts t p ∧ (∀ q' : t.q , (
       rw [←δ']
       exact h w
 
-lemma accepts_suffix_if (l r : word σ) : (∀ q : t.q , reachable t t.init q → δ_star' t q r ∈ t.fs) → dfa_accepts t (l ++ r) := by
+lemma accepts_suffix_if (l r : word t.σs) : (∀ q : t.qs , reachable t t.init q → δ_star' t q r ∈ t.fs) → dfa_accepts t (l ++ r) := by
   intro fa
   simp only [dfa_accepts]
   rw [δ_star_append_eq]
   apply fa
   apply δ_star'_reachable
-  exact reachable.base 
-  
+  exact reachable.base
+
 -- To prove that DFA always accepts some suffix
 -- If from any reachable state the word is accepted, it is always accepted
-theorem accepts_suffix_iff (s : word σ) : (∀ p : word σ,  dfa_accepts t (p ++ s)) ↔ (∀ q : t.q , reachable t t.init q → δ_star' t q s ∈ t.fs) := by
+theorem accepts_suffix_iff (s : word t.σs) : (∀ p : word t.σs,  dfa_accepts t (p ++ s)) ↔ (∀ q : t.qs , reachable t t.init q → δ_star' t q s ∈ t.fs) := by
   apply Iff.intro
   · intro fa q rq
     have := Iff.mp (state_reachable_iff t t.init q) rq
@@ -250,13 +215,13 @@ theorem accepts_suffix_iff (s : word σ) : (∀ p : word σ,  dfa_accepts t (p +
 -- Define whether list forms path between start and finish
 -- The elements (vertices) are joined by edges and each vertex exists at most once
 -- The last element must be the target
-def is_path (a z : t.q) (l : List t.q) : Bool := by
+def is_path (a z : t.qs) (l : List t.qs) : Bool := by
   match l with
   | [] => exact decide (a = z)
-  | q :: qs => exact decide (∃ e : σ , t.δ a e = q) && is_path q z qs && decide (q ∉ qs)
+  | q :: qs => exact decide (∃ e : t.σs , t.δ a e = q) && is_path q z qs && decide (q ∉ qs)
 
 
-theorem target_in_path  (l : List t.q) : (a b : t.q) → is_path t a b l → a ≠ b →  b ∈ l := by
+theorem target_in_path  (l : List t.qs) : (a b : t.qs) → is_path t a b l → a ≠ b → b ∈ l := by
   induction l with
   | nil => intro a b pab _; simp [is_path] at pab; contradiction
   | cons e es s => intro a b pab _;
@@ -269,12 +234,12 @@ theorem target_in_path  (l : List t.q) : (a b : t.q) → is_path t a b l → a �
                    | inr h => apply List.mem_cons.mpr
                               apply Or.inr
                               apply this
-                              simp only [·≠· ]
+                              simp only [·≠·]
                               intro d
                               rw [d] at h
                               contradiction
 
-lemma all_in_path_reachable (l : List t.q) : (a b : t.q) → is_path t a b l → ∀ q : t.q, q ∈ l → reachable t a q := by
+lemma all_in_path_reachable (l : List t.qs) : (a b : t.qs) → is_path t a b l → ∀ q : t.qs, q ∈ l → reachable t a q := by
   induction l with
   | nil => intro a b _ q qin; contradiction
   | cons e es s => intro a b p q qinees
@@ -285,22 +250,26 @@ lemma all_in_path_reachable (l : List t.q) : (a b : t.q) → is_path t a b l →
                                                                exact p.1.2
                                                                exact qines
                               have rae : reachable t a e := by apply Exists.elim (p.1.1)
-                                                               intro s δs 
+                                                               intro s δs
                                                                apply (Iff.mpr (state_reachable_iff t a e))
-                                                               exists [s]
+                                                               apply Exists.elim δs
+                                                               intro sin δ
+                                                               exists [⟨s, sin⟩]
                               apply reachable.trans
                               · exact rae
-                              · exact req 
+                              · exact req
                    | inl h => simp [is_path] at p
                               apply (Iff.mpr (state_reachable_iff t a q))
                               rw [←h] at p
                               apply Exists.elim p.1.1
                               intro s δs
-                              exists [s]
-                   
+                              apply Exists.elim δs
+                              intro sin δ
+                              exists [⟨s, sin⟩]
+
 
 -- Gets all elements from list until it encouters an element (includes the element in result)
-def list_until {α : Type _} (a : α) [DecidableEq α] : List α → List α 
+def list_until {α : Type _} (a : α) [DecidableEq α] : List α → List α
   | [] => []
   | e::es => if e=a then [e] else e::list_until a es
 
@@ -324,18 +293,18 @@ def nin_list_nin_list_until {α : Type _} [DecidableEq α] (a : α) (l : List α
                         · exact this
                         · exact ain
 
-lemma path_if_list_until (l : List t.q) : (a b : t.q) → is_path t a b l → ∀ q : t.q, q ∈ l → is_path t a q (list_until q l) := by
+lemma path_if_list_until (l : List t.qs) : (a b : t.qs) → is_path t a b l → ∀ q : t.qs, q ∈ l → is_path t a q (list_until q l) := by
   induction l with
   | nil => intro a b _ q qin; contradiction
-  | cons e es s => intro a b pab q qin 
+  | cons e es s => intro a b pab q qin
                    simp [is_path] at pab
                    simp only [list_until]
-                   split 
+                   split
                    · simp [is_path]
                      apply And.intro
                      · exact pab.1.1
                      · assumption
-                   · simp [is_path]  
+                   · simp [is_path]
                      apply And.intro
                      · apply And.intro
                        · exact pab.1.1
@@ -350,9 +319,9 @@ lemma path_if_list_until (l : List t.q) : (a b : t.q) → is_path t a b l → �
                              exact qin
                      · apply nin_list_nin_list_until
                        exact pab.2
-                   
 
-lemma all_in_path_path (l : List t.q) : (a b : t.q) → is_path t a b l → ∀ q : t.q, q ∈ l → ∃ l₁ : List t.q, is_path t a q l₁ := by
+
+lemma all_in_path_path (l : List t.qs) : (a b : t.qs) → is_path t a b l → ∀ q : t.qs, q ∈ l → ∃ l₁ : List t.qs, is_path t a q l₁ := by
   match l with
   | [] => intro a b _ q qin; contradiction
   | e::es => intro a b p q qin
@@ -362,12 +331,16 @@ lemma all_in_path_path (l : List t.q) : (a b : t.q) → is_path t a b l → ∀ 
              · exact qin
 
 
-lemma path_concat (l : List t.q) : (a b c : t.q) → is_path t a b l → (∃ e : σ , t.δ b e = c) → c ∉ l → is_path t a c (l.concat c) := by
+lemma path_concat (l : List t.qs) : (a b c : t.qs) → is_path t a b l → (∃ e : t.σs, t.δ b e = c) → c ∉ l → is_path t a c (l.concat c) := by
   induction l with
   | nil => intro a b c p ex cin
            simp [is_path]
-           simp[is_path] at p
-           rw [←p] at ex; exact ex
+           simp [is_path] at p
+           rw [←p] at ex
+           apply Exists.elim ex
+           intro e δ
+           exists e
+           exists e.2
   | cons e es s => intro a b c p ex cin
                    simp [is_path]
                    simp [is_path] at p
@@ -386,7 +359,7 @@ lemma path_concat (l : List t.q) : (a b c : t.q) → is_path t a b l → (∃ e 
                        apply this
                        rw [ec]
 
-theorem reachable_iff_ex_path (a b : t.q) : reachable t a b ↔ ∃ l : List t.q , is_path t a b l := by
+theorem reachable_iff_ex_path (a b : t.qs) : reachable t a b ↔ ∃ l : List t.qs , is_path t a b l := by
   apply Iff.intro
   . intro r
     induction r with
@@ -411,60 +384,42 @@ theorem reachable_iff_ex_path (a b : t.q) : reachable t a b ↔ ∃ l : List t.q
     | inl h => rw [h]; exact reachable.base
     | inr h => apply all_in_path_reachable
                · exact pab
-               · simp [is_path] at pab
+               · simp only [is_path] at pab
                  apply target_in_path
-                 exact pab 
+                 exact pab
                  exact h
 
-    
-theorem path_Nodup (l : List t.q) : (a b : t.q) → is_path t a b l → l.Nodup := by
+
+theorem path_nodup (l : List t.qs) : (a b : t.qs) → is_path t a b l → l.Nodup := by
   induction l with
   | nil => simp
   | cons e es s => intro a b h
-                   simp only [is_path] at h
-                   simp
-                   simp at h
+                   simp [is_path] at h
+                   simp only [List.nodup_cons]
                    apply And.intro
                    · apply h.2
                    · apply s
                      · exact h.1.2
 
-
-theorem path_le_card (l : List t.q) : (a b : t.q) → is_path t a b l → l.card ≤ List.card t.fq.toList := by
+lemma path_finset_subset (l : List t.qs) : (a b : t.qs) → is_path t a b l → l.toFinset ⊆ t.qs.attach := by
   intro a b _
-  apply List.card_subset_le
-  simp [·⊆·, List.Subset]
-  
+  simp only [· ⊆ · ]
+  intro e _
+  apply Finset.mem_attach
 
-theorem card_nodup_eq_len [DecidableEq α ] {l : List α} {nd : l.Nodup} : l.card = l.length := by
-  induction l with
-  | nil => simp
-  | cons a as s => simp only [List.card, List.length]
-                   split
-                   · have ain : a ∈ as := by assumption
-                     have : False := (List.nodup_cons.mp nd).left ain
-                     contradiction
-                   · simp only [·+·,Add.add, Nat.add]
-                     apply congr_arg
-                     apply s
-                     exact (List.nodup_cons.mp nd).right
-
-theorem path_le_size (l : List t.q) : (a b : t.q) → is_path t a b l → l.length ≤ List.length t.fq.toList := by
+theorem path_le_size (l : List t.qs) : (a b : t.qs) → is_path t a b l → l.length ≤ t.qs.card := by
   intro a b pab
-  have h₁ : l.Nodup := path_Nodup t l a b pab 
-  have h₂ : List.Nodup t.fq.toList := FinEnum.nodup_toList
-  rw [←card_nodup_eq_len]
-  rw [←card_nodup_eq_len]
-  apply path_le_card
-  · exact pab
-  · assumption
-  · assumption
+  rw [←Finset.card_attach,←List.toFinset_card_of_nodup]
+  apply Finset.card_le_of_subset
+  apply path_finset_subset
+  exact pab
+  apply path_nodup
+  exact pab
 
 
-instance DecidableIsPath : (a b : t.q) → Decidable (∃ l : List t.q, is_path t a b l) := by
+instance DecidableIsPath : (a b : t.qs) → Decidable (∃ l : List t.qs, is_path t a b l) := by
   intro a b
-  have fin : Fintype t.q := ⟨ List.toFinset t.fq.toList, by simp⟩ 
-  have f : Fintype {l : List t.q // l.Nodup} := @fintypeNodupList t.q t.fq.decEq fin
+  have f : Fintype {l : List t.qs // l.Nodup} := @fintypeNodupList t.qs _ _
   have h : Decidable (∃ l, l ∈ f.elems ∧ (fun l => is_path t a b l) l) := Finset.decidableExistsAndFinset
   match h with
   | isTrue t => apply isTrue
@@ -477,18 +432,16 @@ instance DecidableIsPath : (a b : t.q) → Decidable (∃ l : List t.q, is_path 
                  apply g
                  apply Exists.elim ex
                  intro l la
-                 exists ⟨l , path_Nodup t l a b la⟩
+                 exists ⟨l , path_nodup t l a b la⟩
                  apply And.intro
                  · apply f.complete
                  · simp only [List.Nodup]
                    exact la
 
-
 instance DecidableReachable : DecidableRel (reachable t) := by
   intro a b
-  apply decidable_of_iff (∃ l : List t.q, is_path t a b l)
+  apply decidable_of_iff (∃ l : List t.qs, is_path t a b l)
   apply Iff.symm
   apply reachable_iff_ex_path
-
 
 end DFA
