lean4/Automaton/DFA/Minimization.lean
@@ -6,34 +6,31 @@ open DFA Finset
 
 namespace DFA
 
-variable {σ : Type _} [FinEnum σ] (t : DFA σ)
+variable {σ : Type _} {q : Type _} (r s t : DFA σ q) [DecidableEq σ] [DecidableEq q]
 
 @[simp]
-def minimization_reachable_q : Finset t.q := by
-  have qs := (finenum_to_finset t.q).filter (fun q => reachable t t.init q)
-  exact qs
+def minimization_reachable_q : Finset t.qs := t.qs.attach.filter (fun q => reachable t t.init q)
 
 @[simp]
 def minimization_reachable_init : { x // x ∈ minimization_reachable_q t } := by
-  exact ⟨t.init , by simp [finenum_to_finset]; exact reachable.base⟩ 
+  exact ⟨t.init , by simp [finenum_to_finset]; exact reachable.base⟩
 
 @[simp]
 def minimization_reachable_fs : Finset {x // x ∈ minimization_reachable_q t} := by
   have := Finset.attach (minimization_reachable_q t)
   exact this.filter (fun q => q.1 ∈ t.fs)
 
-
 @[simp]
-def minimization_reachable_δ : { x // x ∈ minimization_reachable_q t } → σ → { x // x ∈ minimization_reachable_q t } := by
+def minimization_reachable_δ : { x // x ∈ minimization_reachable_q t } → t.σs → { x // x ∈ minimization_reachable_q t } := by
   intro q e
   have := q.2
   simp [finenum_to_finset] at this
-  exact ⟨ t.δ q e, by simp [finenum_to_finset]; apply reachable.step; exact this⟩ 
+  exact ⟨ t.δ q e, by simp [finenum_to_finset]; apply reachable.step; exact this⟩
 
-def minimization_reachable : DFA σ := 
-  {q := minimization_reachable_q t, init := minimization_reachable_init t, fs := minimization_reachable_fs t, δ := minimization_reachable_δ t}
+def minimization_reachable : DFA σ {x // x ∈ t.qs} :=
+  {qs := minimization_reachable_q t, init := minimization_reachable_init t, fs := minimization_reachable_fs t, δ := minimization_reachable_δ t}
 
-lemma minimization_reachable_δ_star'_eq (w : word σ) : (q : t.q) → (r : reachable t t.init q) → δ_star' t q w = (δ_star' (minimization_reachable t) ⟨q, by simp [finenum_to_finset]; exact r⟩  w).1 := by
+lemma minimization_reachable_δ_star'_eq (w : word t.σs) : (q : t.qs) → (r : reachable t t.init q) → δ_star' t q w = (δ_star' (minimization_reachable t) ⟨q, by simp [finenum_to_finset, minimization_reachable]; exact r⟩  w).1 := by
   induction w with
   | nil => simp
   | cons a as s => simp only [δ_star']
@@ -43,24 +40,24 @@ lemma minimization_reachable_δ_star'_eq (w : word σ) : (q : t.q) → (r : reac
                    apply reachable.step
                    exact r
 
-theorem minimization_reachable_δ_star_eq (w : word σ) : δ_star t w = (δ_star (minimization_reachable t) w).1 := by
+theorem minimization_reachable_δ_star_eq (w : word t.σs) : δ_star t w = (δ_star (minimization_reachable t) w).1 := by
   simp only [δ_star]
   apply minimization_reachable_δ_star'_eq
   exact reachable.base
 
-theorem minimization_reachable_eq (w : word σ) : dfa_accepts t w ↔ dfa_accepts (minimization_reachable t) w := by
+theorem minimization_reachable_eq (w : word t.σs) : dfa_accepts t w ↔ dfa_accepts (minimization_reachable t) w := by
   apply Iff.intro
   · intro dfa
     simp only [dfa_accepts] at dfa
-    simp only [dfa_accepts] 
+    simp only [dfa_accepts]
     simp [minimization_reachable]
     rw [minimization_reachable_δ_star_eq] at dfa
     simp [minimization_reachable] at dfa
     exact dfa
   · intro dfa
     simp only [dfa_accepts] at dfa
-    simp only [dfa_accepts] 
-    rw [minimization_reachable_δ_star_eq] 
+    simp only [dfa_accepts]
+    rw [minimization_reachable_δ_star_eq]
     simp [minimization_reachable] at dfa
     simp [minimization_reachable]
     exact dfa
