lean4/Automaton/DFA/ToNFA.lean
@@ -13,56 +13,50 @@ open DFA NFA
 
 namespace ToNFA
 
-variable {σ : Type _} [FinEnum σ] (td sd : DFA σ) (tn sn : NFA σ)
+variable {σ : Type _} [DecidableEq σ]  {q : Type _} [DecidableEq q]  (td sd : DFA σ q) (tn sn : NFA σ q)
 
--- dfa and nfa accept the same language
-def dfa_nfa_eq : Prop := ∀ w : word σ , nfa_accepts tn w ↔ dfa_accepts td w
 
 -- to convert into nfa δ, just create singleton for each state
-def dfa_δ_to_nfa_δ : td.q → σ → Finset td.q := λ q e => {td.δ q e}
+def dfa_δ_to_nfa_δ : td.qs → td.σs → Finset td.qs := λ q e => {td.δ q e}
 
 -- conversion from nfa to dfa
-def dfa_to_nfa : NFA σ := by
-  exact {q := td.q , init := td.init , fs := td.fs , δ := dfa_δ_to_nfa_δ td : NFA σ}
+def dfa_to_nfa : NFA σ q := by
+  exact {qs := td.qs , init := td.init , fs := td.fs , δ := dfa_δ_to_nfa_δ td : NFA σ q}
 
 -- the initial state in NFA is same as in the original DFA
-theorem dfa_to_nfa_eq_init : td.init = (dfa_to_nfa td).init := by dsimp [dfa_to_nfa]
+theorem dfa_to_nfa_eq_init : td.init = (dfa_to_nfa td).init := by simp [dfa_to_nfa]
 
 -- the final states of the converted dfa are the same
-theorem dfa_to_nfa_eq_final : td.fs = (dfa_to_nfa td).fs := by dsimp[dfa_to_nfa]
+theorem dfa_to_nfa_eq_final : td.fs = (dfa_to_nfa td).fs := by simp[dfa_to_nfa]
 
 -- the δ_star function remains the same (but NFA produces singletons)
-theorem dfa_to_nfa_eq_δ_star' (w : word σ) : (q : td.q) → {DFA.δ_star' td q w} = NFA.δ_star' (dfa_to_nfa td) {q} w := by
+theorem dfa_to_nfa_eq_δ_star' (w : word td.σs) : (q : td.qs) → {DFA.δ_star' td q w} = NFA.δ_star' (dfa_to_nfa td) {q} w := by
   induction w with
   | nil => intro q; simp [DFA.δ_star,NFA.δ_star]
   | cons a as h => intro q
                    simp [DFA.δ_star,NFA.δ_star]
                    rw [h]
-                   simp [δ_step,dfa_to_nfa,dfa_δ_to_nfa_δ]     
+                   simp [δ_step,dfa_to_nfa,dfa_δ_to_nfa_δ]
 
-theorem dfa_to_nfa_eq_δ_star (w : word σ) : {DFA.δ_star td w} = NFA.δ_star (dfa_to_nfa td) w := by
+theorem dfa_to_nfa_eq_δ_star (w : word td.σs) : {DFA.δ_star td w} = NFA.δ_star (dfa_to_nfa td) w := by
   simp [DFA.δ_star, NFA.δ_star]
   have h : (dfa_to_nfa td).init = td.init := by simp [dfa_to_nfa]
   rw [h]
   apply dfa_to_nfa_eq_δ_star'
 
 -- converted dfa accepts the same language as the original dfa
-theorem dfa_to_nfa_eq : dfa_nfa_eq td (dfa_to_nfa td) := by
-  dsimp [dfa_nfa_eq]
-  intro w
+theorem dfa_to_nfa_eq : dfa_accepts td w ↔ nfa_accepts (dfa_to_nfa td) w := by
+  simp only [dfa_accepts,nfa_accepts,DFA.δ_star,NFA.δ_star]
   apply Iff.intro
-  · intro h
-    rw [←(dfa_to_nfa_eq_δ_star' td w)] at h
-    apply Finset.nonempty_inter_singleton_imp_in
-    exact h
   · intro h
     rw [←(dfa_to_nfa_eq_δ_star' td w)]
     simp only [dfa_to_nfa]
-    rw [DFA.δ_star] at h
-    rw [Finset.singleton_inter_of_mem h]
-    exact (Finset.singleton_nonempty (DFA.δ_star td w))
-
+    apply Finset.in_nonempty_inter_singleton
+    exact h
+  · intro h
+    rw [←(dfa_to_nfa_eq_δ_star' td w)] at h
+    simp only [dfa_to_nfa]
+    apply Finset.nonempty_inter_singleton_imp_in
+    exact h
 
 end ToNFA
-
-
