lean4/Automaton/NFA/Basic.lean
@@ -11,37 +11,39 @@ import Mathlib.Data.FinEnum
 
 namespace NFA
 
-structure NFA (σ : Type _) where
-  q : Type _             -- states
-  init : q               -- initial state
-  fs : Finset q          -- accepting states
-  δ : q → σ → Finset q   -- transition function
-  [fq : FinEnum q]
-  [fσ : FinEnum σ]
+structure NFA (σ : Type _) (q : Type _) where
+  σs : Finset σ    -- alphabet
+  qs : Finset q    -- states
+  init : qs        -- initial state
+  fs : Finset qs   -- accepting states
+  δ : qs → σs → Finset qs -- transition function
+  [dq : DecidableEq q]
+  [dσ : DecidableEq σ]
 
-variable {σ : Type _} (t : NFA σ)
+variable {σ : Type _} {q : Type _}  (r s t : NFA σ q) [DecidableEq σ] [DecidableEq q]
 
-instance : FinEnum t.q := t.fq
+instance : DecidableEq t.σs := by infer_instance
+instance : DecidableEq t.qs := by infer_instance
 
 -- one step in the operation of NFA, consuming one character
 -- take the union of all sets of states reachable from current set of states
 @[simp]
-def δ_step  (q : Finset t.q) (e : σ) : Finset t.q := q.biUnion (fun n => t.δ n e)
+def δ_step  (q : Finset t.qs) (e : t.σs) : Finset t.qs := q.biUnion (fun n => t.δ n e)
 
 -- δ* function for NFA
 -- returns set of states reached after inputting a word
 @[simp]
-def δ_star' (q : Finset t.q) : (w : word σ) → Finset t.q
+def δ_star' (q : Finset t.qs) : (w : word t.σs) → Finset t.qs
   | [] => q
   | e :: es => δ_star' (δ_step t q e) es
 
 @[simp]
-def δ_star : (w : word σ) → Finset t.q := δ_star' t {t.init}
+def δ_star : (w : word t.σs) → Finset t.qs := δ_star' t {t.init}
 
 -- Whether a word is in the language that the NFA accepts
 @[simp]
-def nfa_accepts (w : word σ) : Prop := by
-  have inter : Finset t.q := (δ_star t w) ∩ t.fs
+def nfa_accepts (w : word t.σs) : Prop := by
+  have inter : Finset t.qs := (δ_star t w) ∩ t.fs
   exact inter.Nonempty
 
 -- nfa accepts nil iff init is final
@@ -56,7 +58,7 @@ theorem nfa_accepts_nil_iff_final : nfa_accepts t [] ↔ t.init ∈ t.fs := by
     rw [Finset.singleton_inter_of_mem e]
     exact (Finset.singleton_nonempty t.init)
 
-instance decidableLang (w : word σ) : Decidable (nfa_accepts t w) := by
+instance decidableLang (w : word t.σs) : Decidable (nfa_accepts t w) := by
   dsimp [nfa_accepts]
   apply Finset.decidableNonempty
 
