lean4/Automaton/NFA/ToDFA.lean
@@ -12,20 +12,17 @@ open NFA DFA Finset
 
 namespace ToDFA
 
-variable {σ : Type _} [FinEnum σ] (tn : NFA σ)
+variable {σ : Type _} {q : Type _} [DecidableEq σ] [DecidableEq q] (r s tn : NFA σ q)
 
 @[simp]
-def nfa_to_dfa_q : Finset (Finset tn.q) := by
-  have qs : Finset tn.q := finenum_to_finset tn.q
-  exact qs.powerset
+def nfa_to_dfa_q : Finset (Finset tn.qs) := tn.qs.attach.powerset
 
 @[simp]
-theorem all_in_q (q : Finset tn.q) : q ∈ nfa_to_dfa_q tn := by
+theorem all_in_q (q : Finset tn.qs) : q ∈ nfa_to_dfa_q tn := by
   simp [nfa_to_dfa_q,finenum_to_finset, · ⊆ ·]
 
 @[simp]
-def nfa_to_dfa_init : { x // x ∈ nfa_to_dfa_q tn } := 
-  ⟨{tn.init} , all_in_q tn {tn.init}⟩ 
+def nfa_to_dfa_init : { x // x ∈ nfa_to_dfa_q tn } := ⟨{tn.init} , all_in_q tn {tn.init}⟩ 
 
 @[simp]
 def nfa_to_dfa_fs : Finset { x // x ∈ nfa_to_dfa_q tn } := by
@@ -34,15 +31,15 @@ def nfa_to_dfa_fs : Finset { x // x ∈ nfa_to_dfa_q tn } := by
   intro q
   exact {⟨q , all_in_q tn q⟩}
   
-def nfa_to_dfa_δ : { x // x ∈ nfa_to_dfa_q tn } → σ → { x // x ∈ nfa_to_dfa_q tn } := by
+def nfa_to_dfa_δ : { x // x ∈ nfa_to_dfa_q tn } → tn.σs → { x // x ∈ nfa_to_dfa_q tn } := by
   intro q e
-  have q₁ : Finset tn.q := q.1.biUnion (fun q => tn.δ q e)
+  have q₁ : Finset tn.qs := q.1.biUnion (fun q => tn.δ q e)
   exact ⟨q₁ , all_in_q tn q₁⟩
 
-def nfa_to_dfa : DFA σ := 
-  {q := nfa_to_dfa_q tn, init := nfa_to_dfa_init tn, fs := nfa_to_dfa_fs tn , δ := nfa_to_dfa_δ tn} 
+def nfa_to_dfa : DFA σ (Finset {x // x ∈ tn.qs}) := 
+  {qs := nfa_to_dfa_q tn, σs := tn.σs,  init := nfa_to_dfa_init tn, fs := nfa_to_dfa_fs tn , δ := nfa_to_dfa_δ tn} 
 
-theorem δ_star_eq' : (q : Finset tn.q) → ⟨(NFA.δ_star' tn q w) , all_in_q tn (NFA.δ_star' tn q w)⟩ = DFA.δ_star' (nfa_to_dfa tn) ⟨ q , (all_in_q tn q)⟩  w := by
+theorem δ_star_eq' : (q : Finset tn.qs) → ⟨(NFA.δ_star' tn q w) , all_in_q tn (NFA.δ_star' tn q w)⟩ = DFA.δ_star' (nfa_to_dfa tn) ⟨ q , (all_in_q tn q)⟩  w := by
   induction w with
   | nil => simp [NFA.δ_star,DFA.δ_star,nfa_to_dfa]
   | cons a as s => intro q
@@ -51,7 +48,7 @@ theorem δ_star_eq' : (q : Finset tn.q) → ⟨(NFA.δ_star' tn q w) , all_in_q 
 theorem δ_star_eq : ⟨(NFA.δ_star tn w) , all_in_q tn (NFA.δ_star tn w)⟩ = DFA.δ_star (nfa_to_dfa tn) w := by
   apply δ_star_eq'
 
-theorem nfa_to_dfa_eq (w : word σ) : nfa_accepts tn w ↔ dfa_accepts (nfa_to_dfa tn) w := by
+theorem nfa_to_dfa_eq (w : word tn.σs) : nfa_accepts tn w ↔ dfa_accepts (nfa_to_dfa tn) w := by
   simp only [nfa_accepts,dfa_accepts]
   apply Iff.intro
   · intro a
