lean4/Automaton/DFA/Examples.lean
@@ -10,82 +10,17 @@ import Mathlib.Data.Fin.Basic
 open Nat DFA
 
 
-def δ₁ : Fin 2 → Fin 2 → Fin 2
-  | 0 , 1 => 1
-  | 0 , 0 => 0
-  | 1 , 1 => 1
-  | 1 , 0 => 0
+def δ₁ : { x : Fin 2 // x ∈ ({0 , 1} : Finset (Fin 2)) } → { x : Fin 2 // x ∈ ({0 , 1} : Finset (Fin 2)) } → { x : Fin 2 // x ∈ ({0 , 1} : Finset (Fin 2))}
+  | ⟨0,_⟩ , ⟨1,_⟩ => ⟨1, by simp⟩
+  | ⟨0,_⟩ , ⟨0,_⟩ => ⟨0, by simp⟩
+  | ⟨1,_⟩ , ⟨1,_⟩ => ⟨1, by simp⟩
+  | ⟨1,_⟩ , ⟨0,_⟩ => ⟨0, by simp⟩
 
 -- accepts all words that end with '1'
-def last_is_one : DFA (Fin 2) := {q := Fin 2, init := 0 , fs := {1} , δ := δ₁}
+def last_is_one : DFA (Fin 2) (Fin 2) := {qs := {0, 1}, σs := {0,1}, init := ⟨0,by simp⟩ , fs := {⟨1 , by simp⟩} , δ := δ₁}
 
 def w₁ : word (Fin 2) := [ 1, 0 ]
-def w₂ : word (Fin 2) := [ 0 ,1 ]
+def w₂ : word (Fin 2) := [ 0, 1 ]
 def w₃ : word (Fin 2) := [ ]
 
-theorem accepts_all_last_1 (w : word (Fin 2)) : dfa_accepts last_is_one (w ++ [1]) := by
-  apply accepts_suffix_if
-  intro q r
-  simp [last_is_one]
-  simp [last_is_one] at q
-  match q with
-  | 0 => simp
-  | 1 => simp
-
-
-#eval δ_star' last_is_one last_is_one.init w₁ -- 0
-#eval dfa_accepts last_is_one w₁ -- false
-
-#eval δ_star last_is_one w₂ -- 1
-#eval dfa_accepts last_is_one w₂ -- true
-
-#eval δ_star last_is_one w₃ -- 0
-#eval dfa_accepts last_is_one w₃ -- false
-
-
-#eval (last_is_one)
-
--- accepts all words that start with 1
-def δ₂ : Fin 3 → Fin 2 → Fin 3
-  | 0 , 1 => 1
-  | 0 , 0 => 2
-  | 1 , 1 => 1
-  | 1 , 0 => 1
-  | _ , _ => 2
-
-def first_is_one : DFA (Fin 2) := {q := Fin 3, init := 0, fs := {1} , δ := δ₂}
-
-theorem accepts_all_first_1 (w : word (Fin 2)) : dfa_accepts first_is_one ([1] ++ w) := by
-  apply accepts_prefix_if
-  intro q r
-  induction r with
-  | base => simp
-  | step qc rqc e s => simp [first_is_one] at s            
-                       rw [s]
-                       match e with
-                       | 0 => simp
-                       | 1 => simp
-
--- automata that has one unreachable state (3)
-def δ₃ : Fin 5 → Fin 2 → Fin 5
-  | 0 , 1 => 1
-  | 0 , 0 => 2
-  | 1 , 1 => 1
-  | 1 , 0 => 1
-  | _ , _ => 2
-
-def first_is_one_extra : DFA (Fin 2) := {q := Fin 5, init := 0, fs := {1,4} , δ := δ₃}
-
--- original state size
-#eval first_is_one_extra.fq.card -- 5
-
--- the size is only 3 (removes the unreachable state)
-#eval (minimization_reachable first_is_one_extra).fq.card -- 3
-
-#eval (first_is_one_extra)
-#eval (minimization_reachable first_is_one_extra)
-
-#eval reachable first_is_one_extra first_is_one_extra.init (0 : Fin 5) -- true
-#eval reachable first_is_one_extra first_is_one_extra.init (1 : Fin 5) -- true
-#eval reachable first_is_one_extra first_is_one_extra.init (2 : Fin 5) -- true
-#eval reachable first_is_one_extra first_is_one_extra.init (3 : Fin 5) -- false
+#eval last_is_one
