lean4/Automaton/Finset/Basic.lean
@@ -6,7 +6,7 @@ namespace Finset
 
 variable {α β : Type _} [DecidableEq α]
 
-theorem nonempty_inter_singleton_imp_in (e : α) (es : Finset α) : 
+theorem nonempty_inter_singleton_imp_in (e : α) (es : Finset α) :
   Finset.Nonempty ({e} ∩ es) → e ∈ es := by
     intro ne
     have h₁ : e ∉ es → {e} ∩ es = ∅ := Finset.singleton_inter_of_not_mem
@@ -20,16 +20,19 @@ theorem in_nonempty_inter_singleton (e : α) (es : Finset α) : e ∈ es → Fin
   rw [Finset.inter_comm,Finset.inter_singleton_of_mem ein]
   exact Finset.singleton_nonempty e
 
+theorem subtype_of_finset_to_finset {fα : Finset α} : Finset {a  // a ∈ fα} → Finset α := by
+  intro f
+  exact f.map ⟨ fun a => a.1 , by simp [Function.Injective]⟩
 
-def fin_of_subtype_to_subtype_of_subfin {qs : Finset α} (s : Finset { x // x ∈ qs }) : { x // x ⊆ Finset.attach qs } := by 
-  exact ⟨s , fun x => by simp⟩ 
+def fin_of_subtype_to_subtype_of_subfin {qs : Finset α} (s : Finset { x // x ∈ qs }) : { x // x ⊆ Finset.attach qs } := by
+  exact ⟨s , fun x => by simp⟩
 
-def subtype_of_subfin_to_fin_of_subtype {qs : Finset α}  (s : { x // x ⊆ Finset.attach qs }) : (Finset { x // x ∈ qs }) := by 
+def subtype_of_subfin_to_fin_of_subtype {qs : Finset α}  (s : { x // x ⊆ Finset.attach qs }) : (Finset { x // x ∈ qs }) := by
   exact s.1
 
 def subtype_of_sset_subtype {α : Type _} {s ss : Finset α} (e : { x // x ∈ ss}) : ss ⊆ s → { x // x ∈ s} := by
   intro iss
-  exact ⟨e.1 , by simp; apply Finset.mem_of_subset iss; exact e.2⟩ 
+  exact ⟨e.1 , by simp; apply Finset.mem_of_subset iss; exact e.2⟩
 
 
 def finenum_to_finset (α : Type _) [FinEnum α] : Finset α := (FinEnum.toList α).toFinset
